Cpdt/StackMachine: add Typed

lib/Cpdt/StackMachine.v
@@ -135,3 +135,180 @@ Module Untyped.
     Qed.
   End Exp.
 End Untyped.
+
+Module Typed.
+  Set Implicit Arguments.
+
+  Module Ty.
+    Inductive t : Set :=
+    | Nat
+    | Bool.
+
+    Definition denote (ty : t) : Set :=
+      match ty with
+      | Nat => nat
+      | Bool => bool
+      end.
+  End Ty.
+
+  Module Binop.
+    Inductive t : Ty.t -> Ty.t -> Ty.t -> Set :=
+    | Plus : t Ty.Nat Ty.Nat Ty.Nat
+    | Times : t Ty.Nat Ty.Nat Ty.Nat
+    | Eq : forall a, t a a Ty.Bool
+    | Lt : t Ty.Nat Ty.Nat Ty.Bool.
+
+    Definition denote {x y r : Ty.t} (b : t x y r) : Ty.denote x -> Ty.denote y -> Ty.denote r :=
+      match b with
+      | Plus => plus
+      | Times => mult
+      | Eq Ty.Nat => Nat.eqb
+      | Eq Ty.Bool => eqb
+      | Lt => leb
+      end.
+  End Binop.
+
+  Definition tstack := list Ty.t.
+
+  Fixpoint vstack (ts : tstack) : Set :=
+    match ts with
+    | nil => unit
+    | t :: ts' => Ty.denote t * vstack ts'
+    end%type.
+
+  Module Instr.
+    Inductive t : tstack -> tstack -> Set :=
+    | NConst : forall s, nat -> t s (Ty.Nat :: s)
+    | BConst : forall s, bool -> t s (Ty.Bool :: s)
+    | Binop : forall x y r s, Binop.t x y r -> t (x :: y :: s) (r :: s).
+
+    Definition denote {ts ts' : tstack} (i : t ts ts') : vstack ts -> vstack ts' :=
+      match i with
+      | NConst _ n => fun s => (n, s)
+      | BConst _ b => fun s => (b, s)
+      | Binop _ b => fun s =>
+                       let '(arg1, (arg2, s')) := s in
+                       ((Binop.denote b) arg1 arg2, s')
+      end.
+  End Instr.
+
+  Module Prog.
+    Inductive t : tstack -> tstack -> Set :=
+    | Nil : forall s, t s s
+    | Cons : forall s1 s2 s3, Instr.t s1 s2 -> t s2 s3 -> t s1 s3.
+
+    Fixpoint denote {ts ts' : tstack} (p : t ts ts') : vstack ts -> vstack ts' :=
+      match p with
+      | Nil _ => fun s => s
+      | Cons i p' => fun s => denote p' (Instr.denote i s)
+      end.
+
+    Fixpoint concat {ts ts' ts'' : tstack} (p : t ts ts') : t ts' ts'' -> t ts ts'' :=
+      match p with
+      | Nil _ => fun p' => p'
+      | Cons i p1 => fun p' => Cons i (concat p1 p')
+      end.
+
+    Lemma concat_correct :
+      forall ts ts' ts'' (p : Prog.t ts ts') (p' : Prog.t ts' ts'') (s : vstack ts),
+        Prog.denote (Prog.concat p p') s = Prog.denote p' (Prog.denote p s).
+    Proof.
+      induction p.
+      - simpl.
+        reflexivity.
+      - simpl.
+        auto.
+    Qed.
+  End Prog.
+
+  Module Exp.
+    Inductive t : Ty.t -> Set :=
+    | NConst : nat -> t Ty.Nat
+    | BConst : bool ->  t Ty.Bool
+    | Binop : forall x y r, Binop.t x y r -> t x -> t y -> t r.
+
+    Fixpoint denote {x : Ty.t} (e : t x) : Ty.denote x :=
+      match e with
+      | NConst n => n
+      | BConst b => b
+      | Binop b e1 e2 => (Binop.denote b) (denote e1) (denote e2)
+      end.
+
+    Fixpoint compile {x : Ty.t} (e : t x) (ts : tstack) : Prog.t ts (x :: ts) :=
+      match e with
+      | NConst n => Prog.Cons (Instr.NConst _ n) (Prog.Nil _)
+      | BConst b => Prog.Cons (Instr.BConst _ b) (Prog.Nil _)
+      | Binop b e1 e2 =>
+          Prog.concat
+            (compile e2 _)
+            (Prog.concat
+               (compile e1 _)
+               (Prog.Cons (Instr.Binop _ b) (Prog.Nil _)))
+      end.
+
+    Section Examples.
+      Definition nconst := NConst 42.
+      Definition bconst := BConst false.
+      Definition nested := Binop Binop.Times (Binop Binop.Plus (NConst 2) (NConst 2)) (NConst 7).
+      Definition nested_eq := Binop (Binop.Eq Ty.Nat) (Binop Binop.Plus (NConst 2) (NConst 2)) (NConst 7).
+      Definition nested_lt := Binop Binop.Lt (Binop Binop.Plus (NConst 2) (NConst 2)) (NConst 7).
+
+      Example denote_nconst : denote nconst = 42.
+      auto. Qed.
+
+      Example denote_bconst : denote bconst = false.
+      auto. Qed.
+
+      Example denote_nested : denote nested = 28.
+      auto. Qed.
+
+      Example denote_nested_eq : denote nested_eq = false.
+      auto. Qed.
+
+      Example denote_nested_lt : denote nested_lt = true.
+      auto. Qed.
+
+      Example denote_compile_nconst : Prog.denote (compile nconst nil) tt = (42, tt).
+      auto. Qed.
+
+      Example denote_compile_bconst : Prog.denote (compile bconst nil) tt = (false, tt).
+      auto. Qed.
+
+      Example denote_compile_nested : Prog.denote (compile nested nil) tt = (28, tt).
+      auto. Qed.
+
+      Example denote_compile_nested_eq : Prog.denote (compile nested_eq nil) tt = (false, tt).
+      auto. Qed.
+
+      Example denote_compile_nested_lt : Prog.denote (compile nested_lt nil) tt = (true, tt).
+      auto. Qed.
+    End Examples.
+
+    Lemma compile_correct' : forall x (e : t x) ts (s : vstack ts),
+        Prog.denote (compile e ts) s = (Exp.denote e, s).
+    Proof.
+      induction e.
+      - simpl.
+        reflexivity.
+      - simpl.
+        auto.
+      - intros.
+        unfold Prog.denote.
+        unfold compile.
+        repeat rewrite Prog.concat_correct.
+        repeat rewrite IHe2.
+        repeat rewrite Prog.concat_correct.
+        repeat rewrite IHe1.
+        reflexivity.
+    Qed.
+
+    Theorem compile_correct : forall x (e : t x),
+        Prog.denote (compile e nil) tt = (Exp.denote e, tt).
+    Proof.
+      intros.
+      simpl.
+      rewrite compile_correct'.
+      reflexivity.
+    Qed.
+  End Exp.
+End Typed.
